ArkLib/OracleReduction/Composition/LiftContext.lean
@@ -1,0 +1,706 @@
+import ArkLib.OracleReduction.Security.Basic
+import ToMathlib.PFunctor.Basic
+
+/-!
+  ## Lifting (Oracle) Reductions to Larger Contexts
+
+  Sequential composition is usually not enough to represent oracle reductions in a modular way. We
+  also need to formalize **virtual** oracle reductions, which lift reductions from one
+  (virtual / inner) context into the another (real / outer) context.
+
+  This is what is meant when we informally say "apply so-and-so protocol to this quantity (derived
+  from the input statement & witness)".
+
+  Put in other words, we define a mapping between the input-output interfaces of two (oracle)
+  reductions, without changing anything about the underlying reductions.
+
+  Recall that the input-output interface of an oracle reduction consists of:
+  - Input: `OuterStmtIn : Type`, `OuterOStmtIn : ιₛᵢ → Type`, and `OuterWitIn : Type`
+  - Output: `OuterStmtOut : Type`, `OuterOStmtOut : ιₛₒ → Type`, and `OuterWitOut : Type`
+
+  The liftContext is defined as the following mappings of projections / lifts:
+
+  - `projStmt : OuterStmtIn → InnerStmtIn`
+  - `projOStmt : (simulation involving OuterOStmtIn to produce InnerOStmtIn)`
+  - `projWit : OuterWitIn → InnerWitIn`
+  - `liftStmt : OuterStmtIn × InnerStmtOut → OuterStmtOut`
+  - `liftOStmt : (simulation involving InnerOStmtOut to produce OuterOStmtOut)`
+  - `liftWit : OuterWitIn × InnerWitOut → OuterWitOut`
+
+  Note that since completeness & soundness for oracle reductions are defined in terms of the same
+  properties after converting to (non-oracle) reductions, we only need to focus our efforts on the
+  non-oracle case.
+
+  Note that this _exactly_ corresponds to lenses in programming languages / category theory.
+  Namely, liftContext on the inputs correspond to a `view`/`get` operation (our "proj"), while
+  liftContext on the output corresponds to a `modify`/`set` operation (our "lift").
+
+  More precisely, the `proj/lift` operations correspond to a Lens between two monomial polyonmial
+  functors: `OuterCtxIn y^ OuterCtxOut ⇆ InnerCtxIn y^ InnerCtxOut`.
+
+  What are some expected properties of the liftContext (via the connection to lenses)?
+
+  First, we recall the expected properties of lenses:
+
+  1. `get(lens, set(lens, value, store)) = value`
+  2. `set(lens, new, set(lens, old, store)) = set(lens, new, store)`
+  3. `set(lens, get(lens, store), store) = store`
+  4. and more
+
+  What should this mean here?
+  - one property not mentioned above, is that the pre-image of `projInput` should be invariant
+    for `liftOutput`.
+
+  That is, if `projInput(inp1) = projInput(inp2) = inp*`, then `liftOutput(inp1, out)
+  = liftOutput(inp2, out)` for all `out` which is a possible result of running the oracle
+  reduction on `inp*`. This basically implies a decomposition of sorts between the input to be
+  liftContexted.
+-/
+
+open OracleSpec OracleComp ProtocolSpec
+
+section Transport
+
+open scoped NNReal
+
+/-- A lens for liftContexting (non-oracle) statements between outer and inner contexts -/
+class StatementLens (OuterStmtIn OuterStmtOut InnerStmtIn InnerStmtOut : Type) where
+  projStmt : OuterStmtIn → InnerStmtIn
+  liftStmt : OuterStmtIn × InnerStmtOut → OuterStmtOut
+
+/-- A lens for liftContexting oracle statements between outer and inner contexts
+
+We require knowledge of the (non-oracle) input statement in the outer context, along with the
+(non-oracle) output statement in the inner context. -/
+class OStatementLens (OuterStmtIn InnerStmtOut : Type)
+    {Outer_ιₛᵢ : Type} (OuterOStmtIn : Outer_ιₛᵢ → Type) [∀ i, OracleInterface (OuterOStmtIn i)]
+    {Outer_ιₛₒ : Type} (OuterOStmtOut : Outer_ιₛₒ → Type) [∀ i, OracleInterface (OuterOStmtOut i)]
+    {Inner_ιₛᵢ : Type} (InnerOStmtIn : Inner_ιₛᵢ → Type) [∀ i, OracleInterface (InnerOStmtIn i)]
+    {Inner_ιₛₒ : Type} (InnerOStmtOut : Inner_ιₛₒ → Type) [∀ i, OracleInterface (InnerOStmtOut i)]
+  where
+  -- To access an input oracle statement in the inner context, we may simulate it using the input
+  -- (non-oracle) statement of the outer context, along with oracle access to the outer input oracle
+  -- statements
+  projOStmt : QueryImpl [InnerOStmtIn]ₒ
+    (ReaderT OuterStmtIn (OracleComp [OuterOStmtIn]ₒ))
+  -- To get back an output oracle statement in the outer context, we may simulate it using the input
+  -- (non-oracle) statement of the outer context, the output (non-oracle) statement of the inner
+  -- context, along with oracle access to the inner output oracle statements
+  liftOStmt : QueryImpl [OuterOStmtOut]ₒ
+    (ReaderT (OuterStmtIn × InnerStmtOut) (OracleComp [InnerOStmtOut]ₒ))
+
+/-- A lens for liftContexting witnesses between outer and inner contexts -/
+class WitnessLens (OuterWitIn OuterWitOut InnerWitIn InnerWitOut : Type) where
+  projWit : OuterWitIn → InnerWitIn
+  liftWit : OuterWitIn × InnerWitOut → OuterWitOut
+
+/-- A lens for liftContexting between outer and inner contexts of a (non-oracle) reduction -/
+class ContextLens (OuterStmtIn OuterStmtOut InnerStmtIn InnerStmtOut : Type)
+    (OuterWitIn OuterWitOut InnerWitIn InnerWitOut : Type)
+    extends StatementLens OuterStmtIn OuterStmtOut InnerStmtIn InnerStmtOut,
+      WitnessLens OuterWitIn OuterWitOut InnerWitIn InnerWitOut
+
+/-- A lens for liftContexting between outer and inner contexts of an oracle reduction -/
+class OracleContextLens (OuterStmtIn OuterStmtOut InnerStmtIn InnerStmtOut : Type)
+    {Outer_ιₛᵢ : Type} (OuterOStmtIn : Outer_ιₛᵢ → Type) [∀ i, OracleInterface (OuterOStmtIn i)]
+    {Outer_ιₛₒ : Type} (OuterOStmtOut : Outer_ιₛₒ → Type) [∀ i, OracleInterface (OuterOStmtOut i)]
+    {Inner_ιₛᵢ : Type} (InnerOStmtIn : Inner_ιₛᵢ → Type) [∀ i, OracleInterface (InnerOStmtIn i)]
+    {Inner_ιₛₒ : Type} (InnerOStmtOut : Inner_ιₛₒ → Type) [∀ i, OracleInterface (InnerOStmtOut i)]
+    (OuterWitIn OuterWitOut InnerWitIn InnerWitOut : Type) extends
+
+      StatementLens OuterStmtIn OuterStmtOut InnerStmtIn InnerStmtOut,
+
+      OStatementLens OuterStmtIn InnerStmtOut
+        OuterOStmtIn OuterOStmtOut InnerOStmtIn InnerOStmtOut,
+
+      WitnessLens OuterWitIn OuterWitOut InnerWitIn InnerWitOut
+
+/-
+  Recall the interface of an extractor:
+  - Takes in `WitOut`, `StmtIn`, `Transcript`, `QueryLog`
+  (note: no need for `StmtOut` as it can be derived from `StmtIn`, `Transcript`, and `QueryLog`)
+  - Returns `WitIn`
+
+  We need a lens for the extractor as well.
+
+  Assume we have an inner extractor
+    `E : InnerWitOut → InnerStmtIn → Transcript → QueryLog → InnerWitIn`
+
+  We need to derive an outer extractor
+    `E' : OuterWitOut → OuterStmtIn → Transcript → QueryLog → OuterWitIn`
+
+  Note that `Transcript` and `QueryLog` are the same due to the lens only changing the
+  input-output interface, and not the inside (oracle) reduction.
+
+  So, `E' outerWitOut outerStmtIn transcript queryLog` needs to call
+    `E (map to innerWitOut) (projStmt outerStmtIn) transcript queryLog`
+  and then post-process the result, which is some `innerWitIn`, to get some `outerWitIn`.
+
+  This processing is exactly the same as a lens in the opposite direction between the outer and
+  inner witness types.
+-/
+
+/-- Inverse lens between outer and inner witnesses (going the other direction with respect to
+  input-output), for extractors / knowledge soundness.
+-/
+@[reducible]
+def WitnessLensInv (OuterWitIn OuterWitOut InnerWitIn InnerWitOut : Type) :=
+  WitnessLens OuterWitOut OuterWitIn InnerWitOut InnerWitIn
+-- structure ContextLensInv (OuterStmtOut InnerStmtOut : Type)
+--     (OuterWitIn OuterWitOut InnerWitIn InnerWitOut : Type) extends
+--       WitnessLens OuterWitOut OuterWitIn InnerWitOut InnerWitIn where
+--   projStmt : OuterStmtOut → InnerStmtOut
+  -- projWitInv : InnerWitOut → OuterWitOut
+  -- liftWitInv : InnerWitIn × OuterWitOut → OuterWitIn
+
+/-- Conditions for the lens / transformation to preserve completeness
+
+For `lift`, we require compatibility relations between the outer input statement/witness and
+the inner output statement/witness -/
+class ContextLens.IsComplete {OuterStmtIn OuterStmtOut InnerStmtIn InnerStmtOut : Type}
+    {OuterWitIn OuterWitOut InnerWitIn InnerWitOut : Type}
+    (outerRelIn : OuterStmtIn → OuterWitIn → Prop)
+    (innerRelIn : InnerStmtIn → InnerWitIn → Prop)
+    (outerRelOut : OuterStmtOut → OuterWitOut → Prop)
+    (innerRelOut : InnerStmtOut → InnerWitOut → Prop)
+    (compat : OuterStmtIn × OuterWitIn → InnerStmtOut × InnerWitOut → Prop)
+    (lens : ContextLens OuterStmtIn OuterStmtOut InnerStmtIn InnerStmtOut
+                        OuterWitIn OuterWitOut InnerWitIn InnerWitOut) where
+
+  proj_complete : ∀ stmtIn witIn,
+    outerRelIn stmtIn witIn →
+    innerRelIn (lens.projStmt stmtIn) (lens.projWit witIn)
+
+  lift_complete : ∀ outerStmtIn outerWitIn innerStmtOut innerWitOut,
+    outerRelIn outerStmtIn outerWitIn →
+    innerRelOut innerStmtOut innerWitOut →
+    compat (outerStmtIn, outerWitIn) (innerStmtOut, innerWitOut) →
+    outerRelOut (lens.liftStmt (outerStmtIn, innerStmtOut))
+                (lens.liftWit (outerWitIn, innerWitOut))
+
+/-- Conditions for the lens / transformation to preserve soundness -/
+class StatementLens.IsSound {OuterStmtIn OuterStmtOut InnerStmtIn InnerStmtOut : Type}
+    (outerLangIn : Set OuterStmtIn) (outerLangOut : Set OuterStmtOut)
+    (innerLangIn : Set InnerStmtIn) (innerLangOut : Set InnerStmtOut)
+    (compat : OuterStmtIn → InnerStmtOut → Prop)
+    (stmtLens : StatementLens OuterStmtIn OuterStmtOut InnerStmtIn InnerStmtOut) where
+
+  proj_sound : ∀ outerStmtIn,
+    outerStmtIn ∉ outerLangIn → stmtLens.projStmt outerStmtIn ∉ innerLangIn
+
+  lift_sound : ∀ outerStmtIn innerStmtOut,
+    outerStmtIn ∉ outerLangIn →
+    innerStmtOut ∉ innerLangOut →
+    compat outerStmtIn innerStmtOut →
+      stmtLens.liftStmt (outerStmtIn, innerStmtOut) ∉ outerLangOut
+
+/-- Conditions for the lens / transformation to preserve knowledge soundness
+
+(TODO: double-check) -/
+class ContextLens.IsKnowledgeSound
+    {OuterStmtIn OuterStmtOut InnerStmtIn InnerStmtOut : Type}
+    {OuterWitIn OuterWitOut InnerWitIn InnerWitOut : Type}
+    (outerRelIn : OuterStmtIn → OuterWitIn → Prop)
+    (innerRelIn : InnerStmtIn → InnerWitIn → Prop)
+    (outerRelOut : OuterStmtOut → OuterWitOut → Prop)
+    (innerRelOut : InnerStmtOut → InnerWitOut → Prop)
+    (compat : OuterStmtIn × OuterWitIn → InnerStmtOut × InnerWitOut → Prop)
+    (lensInv : WitnessLensInv OuterWitIn OuterWitOut InnerWitIn InnerWitOut)
+    (lens : ContextLens OuterStmtIn OuterStmtOut InnerStmtIn InnerStmtOut
+                        OuterWitIn OuterWitOut InnerWitIn InnerWitOut) where
+
+  /-- Projecting using the inverse lens from outer to inner context preserves satisfaction of
+    relations -/
+  proj_knowledge_sound : ∀ outerStmtIn outerWitIn,
+    outerRelIn outerStmtIn outerWitIn →
+    innerRelIn (lens.projStmt outerStmtIn) (lens.projWit outerWitIn)
+
+  lift_knowledge_sound : ∀ outerStmtIn outerWitIn innerStmtOut innerWitOut,
+    outerRelIn outerStmtIn outerWitIn →
+    innerRelOut innerStmtOut innerWitOut →
+    compat (outerStmtIn, outerWitIn) (innerStmtOut, innerWitOut) →
+    outerRelOut (lens.liftStmt (outerStmtIn, innerStmtOut))
+                (lens.liftWit (outerWitIn, innerWitOut))
+
+/-
+  The above two soundness / knowledge soundness conditions should be sufficient for all notions,
+  i.e. regular, state-restoration, round-by-round, etc.,
+  since we only act on the input-output interface
+-/
+
+variable {n : ℕ} {pSpec : ProtocolSpec n} {ι : Type} {oSpec : OracleSpec ι}
+  {OuterStmtIn OuterWitIn OuterStmtOut OuterWitOut : Type}
+  {InnerStmtIn InnerWitIn InnerStmtOut InnerWitOut : Type}
+  [∀ i, VCVCompatible (pSpec.Challenge i)]
+
+/-- The outer prover after lifting invokes the inner prover on the projected input, and
+  lifts the output -/
+def Prover.liftContext
+    [lens : ContextLens OuterStmtIn OuterStmtOut InnerStmtIn InnerStmtOut
+                        OuterWitIn OuterWitOut InnerWitIn InnerWitOut]
+    (P : Prover pSpec oSpec InnerStmtIn InnerWitIn InnerStmtOut InnerWitOut) :
+      Prover pSpec oSpec OuterStmtIn OuterWitIn OuterStmtOut OuterWitOut where
+  PrvState := fun i => P.PrvState i × OuterStmtIn × OuterWitIn
+  input := fun stmtIn witIn =>
+    ⟨P.input (lens.projStmt stmtIn) (lens.projWit witIn), stmtIn, witIn⟩
+  sendMessage := fun i ⟨prvState, stmtIn, witIn⟩ => do
+    let ⟨msg, prvState'⟩ ← P.sendMessage i prvState
+    return ⟨msg, ⟨prvState', stmtIn, witIn⟩⟩
+  receiveChallenge := fun i ⟨prvState, stmtIn, witIn⟩ chal =>
+    ⟨P.receiveChallenge i prvState chal, stmtIn, witIn⟩
+  output := fun ⟨prvState, stmtIn, witIn⟩ =>
+    let ⟨innerStmtOut, innerWitOut⟩ := P.output prvState
+    ⟨lens.liftStmt (stmtIn, innerStmtOut), lens.liftWit (witIn, innerWitOut)⟩
+
+/-- The outer verifier after lifting invokes the inner verifier on the projected input, and
+  lifts the output -/
+def Verifier.liftContext
+    [lens : StatementLens OuterStmtIn OuterStmtOut InnerStmtIn InnerStmtOut]
+    (V : Verifier pSpec oSpec InnerStmtIn InnerStmtOut) :
+      Verifier pSpec oSpec OuterStmtIn OuterStmtOut where
+  verify := fun stmtIn transcript => do
+    let innerStmtIn := lens.projStmt stmtIn
+    let innerStmtOut ← V.verify innerStmtIn transcript
+    return lens.liftStmt (stmtIn, innerStmtOut)
+
+/-- The outer reduction after lifting is the combination of the lifting of the prover and
+  verifier -/
+def Reduction.liftContext
+    [lens : ContextLens OuterStmtIn OuterStmtOut InnerStmtIn InnerStmtOut
+      OuterWitIn OuterWitOut InnerWitIn InnerWitOut]
+    (R : Reduction pSpec oSpec InnerStmtIn InnerWitIn InnerStmtOut InnerWitOut) :
+      Reduction pSpec oSpec OuterStmtIn OuterWitIn OuterStmtOut OuterWitOut where
+  prover := R.prover.liftContext
+  verifier := R.verifier.liftContext
+
+open Verifier in
+/-- The outer extractor after lifting invokes the inner extractor on the projected input, and
+  lifts the output -/
+def StraightlineExtractor.liftContext
+    (lens : ContextLens OuterStmtIn OuterStmtOut InnerStmtIn InnerStmtOut
+      OuterWitIn OuterWitOut InnerWitIn InnerWitOut)
+    (lensInv : WitnessLensInv OuterWitIn OuterWitOut InnerWitIn InnerWitOut)
+    (E : StraightlineExtractor pSpec oSpec InnerStmtIn InnerWitIn InnerWitOut) :
+      StraightlineExtractor pSpec oSpec OuterStmtIn OuterWitIn OuterWitOut :=
+  fun outerWitOut outerStmtIn fullTranscript proveQueryLog verifyQueryLog =>
+    let innerStmtIn := lens.projStmt outerStmtIn
+    let innerWitOut := lensInv.projWit outerWitOut
+    let innerWitIn := E innerWitOut innerStmtIn fullTranscript proveQueryLog verifyQueryLog
+    lensInv.liftWit (outerWitOut, innerWitIn)
+
+/-- Compatibility relation between the outer input statement and the inner output statement,
+relative to a verifier.
+
+We require that the inner output statement is a possible output of the verifier on the outer
+input statement, for any given transcript. Note that we have to existentially quantify over
+transcripts since we only reference the verifier, and there's no way to get the transcript without
+a prover. -/
+def Verifier.compatStatement {OuterStmtIn OuterStmtOut InnerStmtIn InnerStmtOut : Type}
+    (lens : StatementLens OuterStmtIn OuterStmtOut InnerStmtIn InnerStmtOut)
+    (V : Verifier pSpec oSpec InnerStmtIn InnerStmtOut) :
+      OuterStmtIn → InnerStmtOut → Prop :=
+  fun outerStmtIn innerStmtOut =>
+    innerStmtOut ∈ ⋃ transcript, (V.run (lens.projStmt outerStmtIn) transcript).support
+
+/-- Compatibility relation between the outer input context and the inner output context, relative
+to a reduction.
+
+We require that the inner output context (statement + witness) is a possible output of the reduction
+on the outer input context (statement + witness). -/
+def Reduction.compatContext {OuterStmtIn OuterStmtOut InnerStmtIn InnerStmtOut : Type}
+    {OuterWitIn OuterWitOut InnerWitIn InnerWitOut : Type}
+    (lens : ContextLens OuterStmtIn OuterStmtOut InnerStmtIn InnerStmtOut
+      OuterWitIn OuterWitOut InnerWitIn InnerWitOut)
+    (R : Reduction pSpec oSpec InnerStmtIn InnerWitIn InnerStmtOut InnerWitOut) :
+      OuterStmtIn × OuterWitIn → InnerStmtOut × InnerWitOut → Prop :=
+  fun ⟨outerStmtIn, outerWitIn⟩ innerContextOut =>
+    innerContextOut ∈
+      Prod.fst <$> (R.run (lens.projStmt outerStmtIn) (lens.projWit outerWitIn)).support
+
+/-- The outer state function after lifting invokes the inner state function on the projected
+  input, and lifts the output -/
+def Verifier.StateFunction.liftContext [oSpec.FiniteRange]
+    [lens : StatementLens OuterStmtIn OuterStmtOut InnerStmtIn InnerStmtOut]
+    (outerLangIn : Set OuterStmtIn) (outerLangOut : Set OuterStmtOut)
+    (innerLangIn : Set InnerStmtIn) (innerLangOut : Set InnerStmtOut)
+    (V : Verifier pSpec oSpec InnerStmtIn InnerStmtOut)
+    [lensSound : lens.IsSound outerLangIn outerLangOut innerLangIn innerLangOut
+      (V.compatStatement lens)]
+    (stF : V.StateFunction pSpec oSpec innerLangIn innerLangOut) :
+      V.liftContext.StateFunction pSpec oSpec outerLangIn outerLangOut
+        -- (lens.projStmt ⁻¹' innerLangIn)
+        -- TODO: figure out the right induced language for `OuterStmtOut`
+        -- (lens.liftStmt '' ( (lens.projStmt ⁻¹' innerLangIn).prod innerLangOut)
+where
+  toFun := fun m outerStmtIn transcript =>
+    stF m (lens.projStmt outerStmtIn) transcript
+  toFun_empty := fun stmt hStmt =>
+    stF.toFun_empty (lens.projStmt stmt) (lensSound.proj_sound stmt hStmt)
+  toFun_next := fun m hDir outerStmtIn transcript hStmt msg =>
+    stF.toFun_next m hDir (lens.projStmt outerStmtIn) transcript hStmt msg
+  toFun_full := fun outerStmtIn transcript hStmt => by
+    have h := stF.toFun_full (lens.projStmt outerStmtIn) transcript hStmt
+    simp [Verifier.run, Verifier.liftContext] at h ⊢
+    intro innerStmtOut hSupport
+    apply lensSound.lift_sound
+    · sorry -- Need `outerStmtIn ∉ outerLangIn`, but we don't have this
+    · exact h innerStmtOut hSupport
+    · simp [compatStatement]; exact ⟨transcript, hSupport⟩
+
+section Theorems
+
+/- Theorems about liftContext interacting with reduction execution and security properties -/
+
+section Prover
+
+/- Breaking down the intertwining of liftContext and prover execution -/
+
+/-- Lifting the prover intertwines with the process round function -/
+theorem Prover.liftContext_processRound
+    [lens : ContextLens OuterStmtIn OuterStmtOut InnerStmtIn InnerStmtOut
+                        OuterWitIn OuterWitOut InnerWitIn InnerWitOut]
+    {i : Fin n}
+    (P : Prover pSpec oSpec InnerStmtIn InnerWitIn InnerStmtOut InnerWitOut)
+    {resultRound : OracleComp (oSpec ++ₒ [pSpec.Challenge]ₒ)
+      (pSpec.Transcript i.castSucc × P.liftContext.PrvState i.castSucc)} :
+      (P.liftContext (lens := lens)).processRound i resultRound
+      = do
+        let ⟨transcript, prvState, outerStmtIn, outerWitIn⟩ ← resultRound
+        let ⟨newTranscript, newPrvState⟩ ← P.processRound i (do return ⟨transcript, prvState⟩)
+        return ⟨newTranscript, ⟨newPrvState, outerStmtIn, outerWitIn⟩⟩ := by
+  unfold processRound liftContext
+  simp
+  congr 1; funext
+  split <;> simp
+
+/-- Lemma needed for the proof of `Prover.liftContext_runToRound` -/
+private lemma Prover.bind_map_processRound_pure {i : Fin n}
+    (P : Prover pSpec oSpec InnerStmtIn InnerWitIn InnerStmtOut InnerWitOut)
+    (comp : OracleComp (oSpec ++ₒ [pSpec.Challenge]ₒ)
+        (pSpec.Transcript i.castSucc × P.PrvState i.castSucc))
+    {α : Type} (f : pSpec.Transcript i.succ × P.PrvState i.succ → α) :
+      (do let result ← comp; f <$> P.processRound i (pure result))
+      = f <$> P.processRound i comp := by
+  simp [processRound]
+
+theorem Prover.liftContext_runToRound
+    [lens : ContextLens OuterStmtIn OuterStmtOut InnerStmtIn InnerStmtOut
+                        OuterWitIn OuterWitOut InnerWitIn InnerWitOut]
+    {outerStmtIn : OuterStmtIn} {outerWitIn : OuterWitIn} {i : Fin (n + 1)}
+    (P : Prover pSpec oSpec InnerStmtIn InnerWitIn InnerStmtOut InnerWitOut) :
+      (P.liftContext (lens := lens)).runToRound i outerStmtIn outerWitIn
+      = do
+        let ⟨transcript, prvState⟩ ←
+          P.runToRound i (lens.projStmt outerStmtIn) (lens.projWit outerWitIn)
+        return ⟨transcript, ⟨prvState, outerStmtIn, outerWitIn⟩⟩ := by
+  unfold runToRound
+  induction i using Fin.induction with
+  | zero => simp [liftContext]
+  | succ i ih => simp [liftContext_processRound, ih, bind_map_processRound_pure]
+
+-- Requires more lemmas about `simulateQ` for logging oracles
+theorem Prover.liftContext_runWithLogToRound
+    [lens : ContextLens OuterStmtIn OuterStmtOut InnerStmtIn InnerStmtOut
+                        OuterWitIn OuterWitOut InnerWitIn InnerWitOut]
+    {outerStmtIn : OuterStmtIn} {outerWitIn : OuterWitIn} {i : Fin (n + 1)}
+    (P : Prover pSpec oSpec InnerStmtIn InnerWitIn InnerStmtOut InnerWitOut) :
+      (P.liftContext (lens := lens)).runWithLogToRound i outerStmtIn outerWitIn
+      = do
+        let ⟨transcript, prvState, queryLog⟩ ←
+          P.runWithLogToRound i (lens.projStmt outerStmtIn) (lens.projWit outerWitIn)
+        return ⟨transcript, ⟨prvState, outerStmtIn, outerWitIn⟩, queryLog⟩ := by
+  unfold runWithLogToRound
+  induction i using Fin.induction with
+  | zero => simp [liftContext]
+  | succ i ih => simp [liftContext_runToRound]
+
+/-- Running the lifted outer prover is equivalent to running the inner prover on the projected
+  input, and then integrating the output -/
+theorem Prover.liftContext_run
+    [lens : ContextLens OuterStmtIn OuterStmtOut InnerStmtIn InnerStmtOut
+                        OuterWitIn OuterWitOut InnerWitIn InnerWitOut]
+    {outerStmtIn : OuterStmtIn} {outerWitIn : OuterWitIn}
+    (P : Prover pSpec oSpec InnerStmtIn InnerWitIn InnerStmtOut InnerWitOut) :
+      P.liftContext.run outerStmtIn outerWitIn
+      = do
+        let ⟨innerStmtOut, innerWitOut, fullTranscript⟩ ←
+          P.run (lens.projStmt outerStmtIn) (lens.projWit outerWitIn)
+        return ⟨lens.liftStmt (outerStmtIn, innerStmtOut),
+                lens.liftWit (outerWitIn, innerWitOut),
+                fullTranscript⟩ := by
+  simp only [Prover.run, liftContext_runToRound]
+  simp [liftContext]
+
+/- Lifting the prover intertwines with the runWithLog function -/
+theorem Prover.liftContext_runWithLog
+    [lens : ContextLens OuterStmtIn OuterStmtOut InnerStmtIn InnerStmtOut
+                        OuterWitIn OuterWitOut InnerWitIn InnerWitOut]
+    {outerStmtIn : OuterStmtIn} {outerWitIn : OuterWitIn}
+    (P : Prover pSpec oSpec InnerStmtIn InnerWitIn InnerStmtOut InnerWitOut) :
+      P.liftContext.runWithLog outerStmtIn outerWitIn
+      = do
+        let ⟨innerStmtOut, innerWitOut, fullTranscript, queryLog⟩ ←
+          P.runWithLog (lens.projStmt outerStmtIn) (lens.projWit outerWitIn)
+        return ⟨lens.liftStmt (outerStmtIn, innerStmtOut),
+                lens.liftWit (outerWitIn, innerWitOut),
+                fullTranscript,
+                queryLog⟩ := by
+  simp only [runWithLog, liftContext_runWithLogToRound]
+  simp [liftContext]
+
+end Prover
+
+theorem Reduction.liftContext_run
+    [lens : ContextLens OuterStmtIn OuterStmtOut InnerStmtIn InnerStmtOut
+                        OuterWitIn OuterWitOut InnerWitIn InnerWitOut]
+    {outerStmtIn : OuterStmtIn} {outerWitIn : OuterWitIn}
+    (R : Reduction pSpec oSpec InnerStmtIn InnerWitIn InnerStmtOut InnerWitOut) :
+      R.liftContext.run outerStmtIn outerWitIn = do
+        let ⟨⟨prvInnerStmtOut, innerWitOut⟩, verInnerStmtOut, fullTranscript⟩ ←
+          R.run (lens.projStmt outerStmtIn) (lens.projWit outerWitIn)
+        return ⟨⟨lens.liftStmt (outerStmtIn, prvInnerStmtOut),
+                lens.liftWit (outerWitIn, innerWitOut)⟩,
+                lens.liftStmt (outerStmtIn, verInnerStmtOut),
+                fullTranscript⟩ := by
+  unfold Reduction.run
+  simp [Reduction.liftContext, Prover.liftContext_run, Verifier.liftContext, Verifier.run]
+
+theorem Reduction.liftContext_runWithLog
+    [lens : ContextLens OuterStmtIn OuterStmtOut InnerStmtIn InnerStmtOut
+                        OuterWitIn OuterWitOut InnerWitIn InnerWitOut]
+    {outerStmtIn : OuterStmtIn} {outerWitIn : OuterWitIn}
+    (R : Reduction pSpec oSpec InnerStmtIn InnerWitIn InnerStmtOut InnerWitOut) :
+      R.liftContext.runWithLog outerStmtIn outerWitIn = do
+        let ⟨⟨prvInnerStmtOut, innerWitOut⟩, verInnerStmtOut, fullTranscript, queryLog⟩ ←
+          R.runWithLog (lens.projStmt outerStmtIn) (lens.projWit outerWitIn)
+        return ⟨⟨lens.liftStmt (outerStmtIn, prvInnerStmtOut),
+          lens.liftWit (outerWitIn, innerWitOut)⟩,
+          lens.liftStmt (outerStmtIn, verInnerStmtOut), fullTranscript, queryLog⟩ := by
+  unfold Reduction.runWithLog
+  simp [Reduction.liftContext, Prover.liftContext_runWithLog, Verifier.liftContext, Verifier.run]
+
+variable [oSpec.FiniteRange]
+
+/--
+  Lifting the reduction preserves completeness, assuming the lens satisfies its completeness
+  conditions
+-/
+theorem Reduction.liftContext_completeness
+    {relIn : OuterStmtIn → OuterWitIn → Prop} {relOut : OuterStmtOut → OuterWitOut → Prop}
+    {relIn' : InnerStmtIn → InnerWitIn → Prop} {relOut' : InnerStmtOut → InnerWitOut → Prop}
+    {completenessError : ℝ≥0}
+    [lens : ContextLens OuterStmtIn OuterStmtOut InnerStmtIn InnerStmtOut
+                        OuterWitIn OuterWitOut InnerWitIn InnerWitOut]
+    (R : Reduction pSpec oSpec InnerStmtIn InnerWitIn InnerStmtOut InnerWitOut)
+    [lensComplete : lens.IsComplete relIn relIn' relOut relOut' (R.compatContext lens)]
+    (h : R.completeness relIn' relOut' completenessError) :
+      R.liftContext.completeness relIn relOut completenessError := by
+  unfold completeness at h ⊢
+  intro outerStmtIn outerWitIn hRelIn
+  have hR := h (lens.projStmt outerStmtIn) (lens.projWit outerWitIn)
+    (lensComplete.proj_complete _ _ hRelIn)
+  rw [Reduction.liftContext_run]
+  refine le_trans hR ?_
+  simp
+  refine probEvent_mono ?_
+  intro ⟨innerContextOut, a, b⟩ hSupport ⟨hRelOut, hRelOut'⟩
+  have : innerContextOut ∈
+      Prod.fst <$> (R.run (lens.projStmt outerStmtIn) (lens.projWit outerWitIn)).support := by
+    simp
+    exact ⟨a, b, hSupport⟩
+  simp_all
+  refine lensComplete.lift_complete _ _ _ _ hRelIn hRelOut ?_
+  rw [← hRelOut']
+  simp [compatContext]; exact this
+
+/-- Lifting the reduction preserves soundness, assuming the lens satisfies its soundness
+  conditions -/
+theorem Verifier.liftContext_soundness [Inhabited InnerStmtOut]
+    {outerLangIn : Set OuterStmtIn} {outerLangOut : Set OuterStmtOut}
+    {innerLangIn : Set InnerStmtIn} {innerLangOut : Set InnerStmtOut}
+    {soundnessError : ℝ≥0}
+    [lens : StatementLens OuterStmtIn OuterStmtOut InnerStmtIn InnerStmtOut]
+    (V : Verifier pSpec oSpec InnerStmtIn InnerStmtOut)
+    -- TODO: figure out the right compatibility relation for the IsSound condition
+    [lensSound : lens.IsSound outerLangIn outerLangOut innerLangIn innerLangOut
+      (V.compatStatement lens)]
+    (h : V.soundness innerLangIn innerLangOut soundnessError) :
+      V.liftContext.soundness outerLangIn outerLangOut soundnessError := by
+  unfold soundness Reduction.run at h ⊢
+  -- Note: there is no distinction between `Outer` and `Inner` here
+  intro WitIn WitOut outerWitIn outerP outerStmtIn hOuterStmtIn
+  simp at h ⊢
+  have innerP : Prover pSpec oSpec InnerStmtIn WitIn InnerStmtOut WitOut := {
+    PrvState := outerP.PrvState
+    input := fun _ _ => outerP.input outerStmtIn outerWitIn
+    sendMessage := outerP.sendMessage
+    receiveChallenge := outerP.receiveChallenge
+    output := fun state =>
+      let ⟨outerStmtOut, outerWitOut⟩ := outerP.output state
+      ⟨default, outerWitOut⟩
+  }
+  have : lens.projStmt outerStmtIn ∉ innerLangIn := by
+    apply lensSound.proj_sound
+    exact hOuterStmtIn
+  have hSound := h WitIn WitOut outerWitIn innerP (lens.projStmt outerStmtIn) this
+  refine le_trans ?_ hSound
+  simp [Verifier.liftContext, Verifier.run]
+  -- Need to massage the two `probEvent`s so that they have the same base computation `oa`
+  -- Then apply `lensSound.lift_sound`?
+  sorry
+
+/-
+  Lifting the reduction preserves knowledge soundness, assuming the lens satisfies its
+  knowledge soundness conditions
+-/
+theorem Verifier.liftContext_knowledgeSoundness [Inhabited InnerStmtOut]
+    {outerRelIn : OuterStmtIn → OuterWitIn → Prop} {outerRelOut : OuterStmtOut → OuterWitOut → Prop}
+    {innerRelIn : InnerStmtIn → InnerWitIn → Prop} {innerRelOut : InnerStmtOut → InnerWitOut → Prop}
+    {knowledgeError : ℝ≥0}
+    [lens : ContextLens OuterStmtIn OuterStmtOut InnerStmtIn InnerStmtOut
+                        OuterWitIn OuterWitOut InnerWitIn InnerWitOut]
+    (lensInv : WitnessLensInv OuterWitIn OuterWitOut InnerWitIn InnerWitOut)
+    [lensKnowledgeSound : lens.IsKnowledgeSound outerRelIn innerRelIn outerRelOut innerRelOut
+      (fun _ _ => True) lensInv]
+    (V : Verifier pSpec oSpec InnerStmtIn InnerStmtOut)
+    (h : V.knowledgeSoundness innerRelIn innerRelOut knowledgeError) :
+      V.liftContext.knowledgeSoundness outerRelIn outerRelOut
+        knowledgeError := by
+  unfold knowledgeSoundness at h ⊢
+  obtain ⟨E, h'⟩ := h
+  refine ⟨E.liftContext lens lensInv, ?_⟩
+  intro outerStmtIn outerWitIn outerP
+  simp [StraightlineExtractor.liftContext]
+  let innerP : Prover pSpec oSpec InnerStmtIn InnerWitIn InnerStmtOut InnerWitOut :=
+    {
+      PrvState := outerP.PrvState
+      input := fun _ _ => outerP.input outerStmtIn outerWitIn
+      sendMessage := outerP.sendMessage
+      receiveChallenge := outerP.receiveChallenge
+      output := fun state =>
+        let ⟨outerStmtOut, outerWitOut⟩ := outerP.output state
+        ⟨default, lensInv.projWit outerWitOut⟩
+    }
+  have h_innerP_input {innerStmtIn} {innerWitIn} :
+      innerP.input innerStmtIn innerWitIn = outerP.input outerStmtIn outerWitIn := rfl
+  have hR := h' (lens.projStmt outerStmtIn) (lens.projWit outerWitIn) innerP
+  simp at hR
+  simp [Reduction.runWithLog, Verifier.liftContext, Verifier.run] at hR ⊢
+  have h_innerP_runWithLog {innerStmtIn} {innerWitIn} :
+      innerP.runWithLog innerStmtIn innerWitIn
+      = do
+        let ⟨_, outerWitOut, rest⟩ ← outerP.runWithLog outerStmtIn outerWitIn
+        return ⟨default, lensInv.projWit outerWitOut, rest⟩ := by
+    sorry
+  refine le_trans ?_ hR
+  -- Massage the two `probEvent`s so that they have the same base computation `oa`?
+  simp [h_innerP_runWithLog]
+  -- apply probEvent_mono ?_
+  sorry
+
+/-
+  Lifting the reduction preserves round-by-round soundness, assuming the lens satisfies its
+  soundness conditions
+-/
+theorem Verifier.liftContext_rbr_soundness
+    {outerLangIn : Set OuterStmtIn} {outerLangOut : Set OuterStmtOut}
+    {innerLangIn : Set InnerStmtIn} {innerLangOut : Set InnerStmtOut}
+    {rbrSoundnessError : pSpec.ChallengeIdx → ℝ≥0}
+    [lens : StatementLens OuterStmtIn OuterStmtOut InnerStmtIn InnerStmtOut]
+    (V : Verifier pSpec oSpec InnerStmtIn InnerStmtOut)
+    -- TODO: figure out the right compatibility relation for the IsSound condition
+    [lensSound : lens.IsSound outerLangIn outerLangOut innerLangIn innerLangOut
+      (V.compatStatement lens)]
+    (h : V.rbrSoundness innerLangIn innerLangOut rbrSoundnessError) :
+      V.liftContext.rbrSoundness outerLangIn outerLangOut rbrSoundnessError := by
+  unfold rbrSoundness at h ⊢
+  obtain ⟨stF, h⟩ := h
+  sorry
+
+/-
+  Lifting the reduction preserves round-by-round knowledge soundness, assuming the lens
+  satisfies its knowledge soundness conditions
+-/
+theorem Verifier.liftContext_rbr_knowledgeSoundness
+    {outerRelIn : OuterStmtIn → OuterWitIn → Prop} {outerRelOut : OuterStmtOut → OuterWitOut → Prop}
+    {innerRelIn : InnerStmtIn → InnerWitIn → Prop} {innerRelOut : InnerStmtOut → InnerWitOut → Prop}
+    {rbrKnowledgeError : pSpec.ChallengeIdx → ℝ≥0}
+    [lens : ContextLens OuterStmtIn OuterStmtOut InnerStmtIn InnerStmtOut
+                        OuterWitIn OuterWitOut InnerWitIn InnerWitOut]
+    (lensInv : WitnessLensInv OuterWitIn OuterWitOut InnerWitIn InnerWitOut)
+    [lensKnowledgeSound : lens.IsKnowledgeSound outerRelIn innerRelIn outerRelOut innerRelOut
+      (fun _ _ => True) lensInv]
+    (V : Verifier pSpec oSpec InnerStmtIn InnerStmtOut)
+    (h : V.rbrKnowledgeSoundness innerRelIn innerRelOut rbrKnowledgeError) :
+      V.liftContext.rbrKnowledgeSoundness outerRelIn outerRelOut
+        rbrKnowledgeError := by
+  sorry
+
+end Theorems
+
+
+-- TODO: state definitions & theorems about oracle reduction as well
+
+
+end Transport
+
+section Test
+
+open Polynomial
+
+-- Testing out sum-check-like relations
+
+noncomputable section
+
+def OuterStmtIn_Test := ℤ[X] × ℤ[X] × ℤ
+def InnerStmtIn_Test := ℤ[X] × ℤ
+
+def outerRelIn_Test : OuterStmtIn_Test → Unit → Prop :=
+  fun ⟨p, q, t⟩ _ => ∑ x ∈ {0, 1}, (p * q).eval x = t
+def innerRelIn_Test : InnerStmtIn_Test → Unit → Prop :=
+  fun ⟨f, t⟩ _ => ∑ x ∈ {0, 1}, f.eval x = t
+
+def OuterStmtOut_Test := ℤ[X] × ℤ[X] × ℤ × ℤ
+def InnerStmtOut_Test := ℤ[X] × ℤ × ℤ
+
+def outerRelOut_Test : OuterStmtOut_Test → Unit → Prop :=
+  fun ⟨p, q, t, r⟩ _ => (p * q).eval r = t
+def innerRelOut_Test : InnerStmtOut_Test → Unit → Prop :=
+  fun ⟨f, t, r⟩ _ => f.eval r = t
+
+def testLens :
+    ContextLens OuterStmtIn_Test OuterStmtOut_Test InnerStmtIn_Test InnerStmtOut_Test
+                Unit Unit Unit Unit where
+  projStmt := fun ⟨p, q, t⟩ => ⟨p * q, t⟩
+  liftStmt := fun ⟨⟨p, q, _⟩, ⟨_, t', u⟩⟩ => (p, q, t', u)
+  projWit := fun (_ : Unit) => (() : Unit)
+  liftWit := fun (_ : Unit × Unit) => (() : Unit)
+
+def testLensInv : WitnessLensInv Unit Unit Unit Unit where
+  projWit := fun _ => ()
+  liftWit := fun _ => ()
+
+def testLensComplete : testLens.IsComplete
+      outerRelIn_Test innerRelIn_Test outerRelOut_Test innerRelOut_Test
+      (fun ⟨⟨p, q, _⟩, ()⟩ ⟨⟨f, _⟩, ()⟩ => p * q = f) where
+  proj_complete := fun ⟨p, q, t⟩ () hRelIn => by
+    simp [outerRelIn_Test] at hRelIn
+    simp [innerRelIn_Test, testLens, hRelIn]
+  lift_complete := fun ⟨p, q, t⟩ _ ⟨f, t', r⟩ _ hRelIn hRelOut' hCompat => by
+    simp [outerRelIn_Test] at hRelIn
+    simp [innerRelOut_Test] at hRelOut'
+    simp at hCompat
+    simp [outerRelOut_Test, testLens, hRelIn, ← hRelOut', hCompat]
+
+def testLensKnowledgeSound : testLens.IsKnowledgeSound
+      outerRelIn_Test innerRelIn_Test outerRelOut_Test innerRelOut_Test
+      (fun ⟨⟨p, q, _⟩, ()⟩ ⟨⟨f, _⟩, ()⟩ => p * q = f) testLensInv where
+  proj_knowledge_sound := fun ⟨p, q, t⟩ () hRelIn => by
+    simp [outerRelIn_Test] at hRelIn
+    simp [innerRelIn_Test, testLens, hRelIn]
+  lift_knowledge_sound := fun ⟨p, q, t⟩ _ ⟨f, t', r⟩ _ hRelIn hRelOut' hCompat => by
+    simp [outerRelIn_Test] at hRelIn
+    sorry
+end
+
+end Test
